lib/ModuRes/Util.v
@@ -1,6 +1,5 @@
 Require Import Ssreflect.ssreflect.
 Require Import Setoid SetoidClass.
-Require Import List.
 
 Ltac find_rewrite1 t0 t1 := match goal with
                             | H: t0 = t1 |- _ => rewrite-> H
@@ -18,22 +17,8 @@ Tactic Notation "ddes" constr(T) "at" integer_list(pos) "as" simple_intropattern
 
 Ltac split_conjs := repeat (match goal with [ |- _ /\ _ ] => split end).
 
-(* TODO: Is this already defined somewhere? *)
+(* TODO RJ: Is this already defined somewhere? *)
 Class DecEq (T : Type) := dec_eq : forall (t1 t2: T), {t1 = t2} + {t1 <> t2}.
 
-(* Stuff that ought to be in the stdlib... *)
-Lemma NoDup_app3 {T} (l1 l2 l3: list T):
-  NoDup (l1 ++ l2 ++ l3) -> NoDup (l2 ++ l1 ++ l3).
-Proof.
-  revert l2 l3. induction l1; induction l2; intro l3; simpl; try tauto; [].
-  move=>Hndup. change (NoDup (a0 :: l2 ++ (a::nil) ++ l1 ++ l3)).
-  apply NoDup_cons; last first.
-  - apply IHl2. eapply NoDup_remove_1. eassumption.
-  - rewrite app_comm_cons in Hndup. apply NoDup_remove_2 in Hndup.
-    move=>Hin. apply Hndup. clear -Hin. rewrite !in_app_iff. rewrite ->!in_app_iff in Hin.
-    destruct Hin as [Hin|[[Hin|[]]|[Hin|Hin]]].
-    + right. left. assumption.
-    + left. left. assumption.
-    + left. right. assumption.
-    + right. right. assumption.
-Qed.
+    
+  
